\sektion{3}{Class Lecture 10/1}
\subsektion{Induction}
\textbf{Setting:} we have some statement $P(x)$ and and some fixed $a \in \NN$, we want to show that $\forall n \in \NN ( (n \ge a) \to P(n) )$.
\begin{example}Method:
\begin{enumerate}
\item Base Case: Prove $P(a)$
\item Induction Step: Let $k \ge a$, and we assume $P(k)$. From this, we try to prove $P(k+1)$.
\end{enumerate}
If we can do both 1 and 2, we can conclude $\forall n \in \NN ( (n \ge a) \to P(n) )$
\end{example}
\begin{proof}[Corollary 4.2.6] Let $n \in \NN$. $2^n= \displaystyle\sum^n_{j=0} \Matx{n \\ j}$. This is equivalent to:
\[ 2^n = \Matx{n \\ 0}+\Matx{n \\ 1}+\cdots+\Matx{n \\ n} \]
\end{proof}
\begin{proof}
By induction.
\begin{enumerate}
\item Base Case: $n=0$. $2^0 = 1$, $\therefore\ \Matx{0 \\ 0} = 1$ \checkmark
\item Induction Step: Assume $k \in \NN$. $2^k = \Matx{k \\ 0}+\Matx{k \\ 1}+\cdots+\Matx{k \\ k}$
	\begin{enumerate}
		\item To Show: $2^{k+1} = \Matx{k+1 \\ 0}+\cdots+\Matx{k+1\\k+1}$
		\item \textbf{Notice:} $2^{k+1} = 2^k2 = 2\left( \Matx{k\\0}+\Matx{k\\1}+\cdots+\Matx{k\\k}\right)$
		\item See page 42 in the textbook (Pascal's Identity).
		\begin{enumerate}
			\item $\Matx{k+1\\0} \equiv$
			\item $\Matx{k+1\\1} \equiv  \Matx{k\\0}+\Matx{k\\1}$
			\item $\Matx{k+1\\2} \equiv  \Matx{k\\0}+\Matx{k\\1}+\Matx{k\\2}$
			\item $\Matx{k+1\\k}\equiv   \Matx{k\\k-1}+\Matx{k\\k}$
			\item $\Matx{k+1\\k+1}\equiv \Matx{k\\k}$
			\item Notice that every term has shown up twice!
			\item $\therefore$ $2 \left( \Matx{k\\0}+\Matx{k\\1}+\cdots+\Matx{k\\k} \right) = 2^{k+1}$ \textbf{QED}
		\end{enumerate}
	\end{enumerate}
\end{enumerate}
\end{proof}
\textbf{If a proof or theorem has a name, we should know how to use it.}
\begin{proof}
For $n \ge 2$, $3n > 3+n$. By induction.
\begin{enumerate}
	\item Base Case: $n=2$ $3*2 = 6 > 5 = 3 + 2$ \checkmark
	\item Induction Step: Let $n \ge 2$. Assume $3n > 3 +n$.
		\begin{enumerate}
			\item To Show: $3(n+1)>3+(n+1)$
			\item $3(n+1)=3n+3$.
			\item By induction hypothesis $3n > 3+n$. $\therefore\ 3n+3>(3+n)+3$.
			\item $(3+n)+3=3+(n+3)>3+(n+1)$
			\item $\therefore\ 3(n+1) > 3+(n+1)$
			\item \textbf{QED} for Induction Step.
		\end{enumerate}
\end{enumerate}
\end{proof}
\subsektion{Strong Induction}
\textbf{Setup}: We want to show $\forall n \in \NN ( (n \ge a) \to P(n))$.
\begin{definition}Method:
\begin{enumerate}
\item Base Case: Show $P(a)$
\item Strong Induction Step: Let $k\ge a$. Assume $P(a) \wedge P(a+1)\wedge \cdots \wedge P(k)$.
\end{enumerate}
From this assumption we prove $P(k+1)$.
\end{definition}
\begin{proof}[Theorem 2.2.4]
\[\forall n \in \NN ( n \ge 1 \to \exists p \in \NN ( p \text{ is prime} \wedge p|n)) \]
\begin{enumerate}
\item Base Case: $n = 2$. $2$ is prime and $2|2$ \checkmark
\item Strong Induction Step: Let $k \in \NN, k \ge 2$. Assume that $2,\cdots,k$ all have prime divisors.
\end{enumerate}
\end{proof}


